Remove CSkEnv

cfrontend/CtypesC.v
@@ -11,6 +11,8 @@ Require Import Skeleton ASTC.
 
 Set Implicit Arguments.
 
+Generalizable Variables F.
+
 Definition fundef_of_fundef F (f: Ctypes.fundef F): AST.fundef F :=
   match f with
   | Internal f => AST.Internal f
@@ -27,37 +29,40 @@ Definition globdef_of_globdef F V (gd: globdef (Ctypes.fundef F) V) : globdef (A
   | Gvar v => Gvar v
   end.
 
-Definition is_external F (gd: globdef (Ctypes.fundef F) type): bool :=
-  match gd with
-  | Gfun fd => is_external_fd fd
-  | Gvar _ => false
-  end
-.
+(* Definition is_external F (gd: globdef (Ctypes.fundef F) type): bool := *)
+(*   match gd with *)
+(*   | Gfun fd => is_external_fd fd *)
+(*   | Gvar _ => false *)
+(*   end *)
+(* . *)
 
-Module CSkEnv.
+Global Instance fundef_HasExternal {F}: HasExternal (Ctypes.fundef F) :=
+  Build_HasExternal (fun fd => is_external_fd (fundef_of_fundef fd)).
 
-  Definition revive {F} (skenv: SkEnv.t) (prog: Ctypes.program F): Genv.t (Ctypes.fundef F) type :=
-    skenv.(Genv_map_defs) (fun blk gd => (do id <- skenv.(Genv.invert_symbol) blk;
-                                         do gd <- prog.(prog_defmap) ! id;
-                                         assertion (negb (is_external gd));
-                                         Some gd))
-  .
+(* Module CSkEnv. *)
 
-  Lemma revive_no_external
-        F (prog: Ctypes.program F)
-        skenv blk gd
-        (DEF: Genv.find_def (revive skenv prog) blk = Some gd)
-        (EXTERNAL: is_external gd)
-    :
-      False
-  .
-  Proof.
-    unfold revive in *.
-    apply_all_once Genv_map_defs_def. des.
-    u in *. des_ifs.
-  Qed.
+(*   Definition revive {F} (skenv: SkEnv.t) (prog: Ctypes.program F): Genv.t (Ctypes.fundef F) type := *)
+(*     skenv.(Genv_map_defs) (fun blk gd => (do id <- skenv.(Genv.invert_symbol) blk; *)
+(*                                          do gd <- prog.(prog_defmap) ! id; *)
+(*                                          assertion (negb (is_external gd)); *)
+(*                                          Some gd)) *)
+(*   . *)
 
-End CSkEnv.
+(*   Lemma revive_no_external *)
+(*         F (prog: Ctypes.program F) *)
+(*         skenv blk gd *)
+(*         (DEF: Genv.find_def (revive skenv prog) blk = Some gd) *)
+(*         (EXTERNAL: is_external gd) *)
+(*     : *)
+(*       False *)
+(*   . *)
+(*   Proof. *)
+(*     unfold revive in *. *)
+(*     apply_all_once Genv_map_defs_def. des. *)
+(*     u in *. des_ifs. *)
+(*   Qed. *)
+
+(* End CSkEnv. *)
 
 (* Definition program_of_program' F (p: program F) : AST.program (AST.fundef F) type := *)
 (*   {| AST.prog_defs := map (fun idg => update_snd (@globdef_of_globdef _ _) idg) p.(prog_defs); *)
