compose/Skeleton.v
@@ -8,6 +8,8 @@ Require Import Linking.
 
 Set Implicit Arguments.
 
+Generalizable Variables F.
+
 
 
 Definition is_gvar F V (gd: globdef F V): bool :=
@@ -163,14 +165,14 @@ I think "sim_skenv_monotone" should be sufficient.
   .
 
   (* Note: We only remove definitions. One can still get the address of external identifier. *)
-  Definition revive {F V} (skenv: SkEnv.t) (prog: AST.program (AST.fundef F) V): Genv.t (AST.fundef F) V :=
+  Definition revive `{HasExternal F} {V} (skenv: SkEnv.t) (prog: AST.program F V): Genv.t F V :=
     skenv.(Genv_map_defs) (fun blk gd => (do id <- skenv.(Genv.invert_symbol) blk;
                                             do gd <- prog.(prog_defmap) ! id;
                                             assertion (negb (is_external gd));
                                             Some gd))
   .
 
-  Inductive genv_precise {F V} (ge: Genv.t (AST.fundef F) V) (p: program (AST.fundef F) V): Prop :=
+  Inductive genv_precise `{HasExternal F} {V} (ge: Genv.t F V) (p: program F V): Prop :=
   | genv_compat_intro
       (FIND_MAP: forall id g,
           p.(prog_defmap) ! id = Some g ->
@@ -182,7 +184,7 @@ I think "sim_skenv_monotone" should be sufficient.
   .
 
   Lemma revive_no_external
-        F V (prog: AST.program (AST.fundef F) V)
+        `{HasExternal F} V (prog: AST.program F V)
         skenv blk gd
         (DEF: Genv.find_def (SkEnv.revive skenv prog) blk = Some gd)
         (EXTERNAL: is_external gd)
@@ -196,8 +198,8 @@ I think "sim_skenv_monotone" should be sufficient.
   Qed.
 
   Lemma revive_precise
-        F V
-        skenv (prog: AST.program (AST.fundef F) V)
+        `{HasExternal F} V
+        skenv (prog: AST.program F V)
         (DEFS0: forall id, In id prog.(prog_defs_names) -> is_some (skenv.(Genv.find_symbol) id))
         (WF: wf skenv)
     :
@@ -226,7 +228,7 @@ I think "sim_skenv_monotone" should be sufficient.
       clear_tac.
       inv WF.
       exploit SYMBDEF; eauto. i; des.
-      unfold Genv.find_def in *. rewrite H. cbn.
+      unfold Genv.find_def in *. rewrite H1. cbn.
       apply Genv.find_invert_symbol in Heq.
       des_ifs; ss.
   Qed.
